src/gsim/gSimAux.v
@@ -167,3 +167,20 @@ Section FINALIZED.
     i. inv x4. ss. rewrite EQ. eapply PROMISES in EQ. clarify.
   Qed.
 End FINALIZED.
+
+Lemma memory_init_get_if loc to from msg
+      (GET: Memory.get loc to Memory.init = Some (from, msg))
+  :
+    to = Time.bot /\ from = Time.bot /\ msg = Message.elt.
+Proof.
+  unfold Memory.get, Memory.init in *.
+  erewrite Cell.init_get in GET. des_ifs.
+Qed.
+
+Lemma memory_init_get loc
+  :
+  Memory.get loc Time.bot Memory.init = Some (Time.bot, Message.elt).
+Proof.
+  unfold Memory.get, Memory.init in *.
+  erewrite Cell.init_get. des_ifs.
+Qed.
